bedrock2/src/ExprImp.v
@@ -21,11 +21,10 @@ Section ExprImp1.
   Context {FName : NameWithEq}.
   Notation func := (@name FName).
 
-
-  Context {state: Type}.
-  Context {stateMap: Map state var (word wXLEN)}.
-  Context {vars: Type}.
-  Context {varset: set vars var}.
+  Context {stateMap: MapFunctions var (word wXLEN)}.
+  Notation state := (map var (word wXLEN)).
+  Context {varset: SetFunctions var}.
+  Notation vars := (set var).
 
   Ltac state_calc := state_calc_generic (@name Name) (word wXLEN).
   Ltac set_solver := set_solver_generic (@name Name).
@@ -56,7 +55,10 @@ Section ExprImp1.
     end.
 
   Section WithEnv.
-    Context {env} {funcMap: Map env func (list var * list var * stmt)} (e:env).
+    Context {funcMap: MapFunctions func (list var * list var * stmt)}.
+    Notation env := (map func (list var * list var * stmt)).
+    Context (e: env).
+
     Fixpoint eval_stmt(f: nat)(st: state)(m: mem)(s: stmt): option (state * mem) :=
       match f with
       | 0 => None (* out of fuel *)
@@ -90,11 +92,11 @@ Section ExprImp1.
         | SCall binds fname args =>
           fimpl <- get e fname;
           let '(params, rets, fbody) := fimpl in
-          argvs <- option_all (map (eval_expr st) args);
-          st0 <- putmany params argvs empty;
+          argvs <- option_all (List.map (eval_expr st) args);
+          st0 <- putmany params argvs empty_map;
           st1m' <- eval_stmt f st0 m fbody;
           let '(st1, m') := st1m' in
-          retvs <- option_all (map (get st1) rets);
+          retvs <- option_all (List.map (get st1) rets);
           st' <- putmany binds retvs st;
           Return (st', m')
         end
@@ -178,10 +180,10 @@ Section ExprImp1.
       eval_stmt (S f) st m1 (SCall binds fname args) = Some p2 ->
       exists params rets fbody argvs st0 st1 m' retvs st',
         get e fname = Some (params, rets, fbody) /\
-        option_all (map (eval_expr st) args) = Some argvs /\
-        putmany params argvs empty = Some st0 /\
+        option_all (List.map (eval_expr st) args) = Some argvs /\
+        putmany params argvs empty_map = Some st0 /\
         eval_stmt f st0 m1 fbody = Some (st1, m') /\
-        option_all (map (get st1) rets) = Some retvs /\
+        option_all (List.map (get st1) rets) = Some retvs /\
         putmany binds retvs st = Some st' /\
         p2 = (st', m').
     Proof. inversion_lemma. Qed.
@@ -286,15 +288,18 @@ Section ExprImp2.
   Context {FName: NameWithEq}.
   Notation func := (@name FName).
 
-  Context {state: Type}.
-  Context {stateMap: Map state var (word wXLEN)}.
-  Context {vars: Type}.
-  Context {varset: set vars var}.
+  Context {stateMap: MapFunctions var (word wXLEN)}.
+  Notation state := (map var (word wXLEN)).
+  Context {varset: SetFunctions var}.
+  Notation vars := (set var).
+
+  Context {funcMap: MapFunctions func (list var * list var * @stmt Bw Name FName)}.
+  Notation env := (map func (list var * list var * stmt)).
 
   Ltac state_calc := state_calc_generic (@name Name) (word wXLEN).
 
-  Lemma modVarsSound: forall env fuel s initialS initialM finalS finalM,
-    eval_stmt env fuel initialS initialM s = Some (finalS, finalM) ->
+  Lemma modVarsSound: forall (e: env) fuel s initialS initialM finalS finalM,
+    eval_stmt e fuel initialS initialM s = Some (finalS, finalM) ->
     only_differ initialS (modVars s) finalS.
   Proof.
     induction fuel; introv Ev.
@@ -355,8 +360,12 @@ Definition isRight(x y z: word 32) :=
                                           (EOp OTimes (EVar _b) (EVar _b)))
                                (EOp OTimes (EVar _c) (EVar _c)))).
 
+Definition annoying_eq: DecidableEq
+  (list (@name ZName) * list (@name ZName) * @stmt BitWidth32 ZName ZName). Admitted.
+Existing Instance annoying_eq.
+
 Definition run_isRight(x y z: word 32): option (word 32) :=
-  final <- (eval_stmt empty 10 empty no_mem (isRight x y z));
+  final <- (eval_stmt empty_map 10 empty_map no_mem (isRight x y z));
   let '(finalSt, finalM) := final in
   get finalSt _isRight.
 
